\begin{center}\section{ 并集，交集}\end{center}
\subsection{定义}
\begin{center}
    (\(\vee\) 或,\(\land\) 与) \\
$A\cup B=\{x\in A\vee x\in B\}$ \\
$A\cap B=\{x\in A\land x\in B\}$
\end{center}
\subsection{运算}
$$\begin{cases}
    \mbox{交换律} \begin{cases}
        A\cup B&= B\cup A  \\
        A\cap B&= B\cap A
    \end{cases} \\
    \mbox{结合律}\begin{cases}
        (A\cup B)\cup C = A\cup(B\cup C) \\
        (A\cap B)\cap C = A\cap(B\cap C)
    \end{cases} \\
    \mbox{分配律}\begin{cases}
        (A\cup B)\cap C = (A\cap C)\cup (B \cap C) \\
        (A\cap B)\cup C = (A\cup C)\cap (B \cup C) \\
    \end{cases}\\
    \mbox{对偶律}\begin{cases}
        (A\cup B)^C = A^C\cap B^C \\
        (A\cap B)^C = A^C\cup B^C
    \end{cases}
\end{cases}$$
\begin{center}
    $A\cup A= A = A\cap A $\\
    $A = B \Leftrightarrow A\subset B\land A\supset B$  \\
    $A\cup\varnothing = A {\qquad}A\cap\varnothing = \varnothing $
\end{center}
\subsection{性质}
\begin{equation}
	A\subset(A\cup B) {\qquad}A\supset(A\cap B)
\end{equation}
\begin{align}
	A\cup B = B\Leftrightarrow A\subset B\\
	A\cap B = A\Leftrightarrow A\subset B
\end{align}
\begin{align}
&(n\in N)\quad&A\cup(B_1\cap B_2\cap\cdots\cap B_n) = (A\cup B_1)\cap(A\cup B_2)\cap\cdots\cap(A\cup B_n)\\
&(n\in N)&A\cap(B_1\cup B_2\cup\cdots\cup B_n) = (A\cap B_1)\cup(A\cap B_2)\cup\cdots\cup(A\cap B_n)
\end{align}
\subsection{gustus De Morgan定理}
$$\neg(A\vee B)\Leftrightarrow(\neg A)\land(\neg B)$$
$$\neg(A\land B)\Leftrightarrow(\neg A)\vee(\neg B)$$
\subsection{德摩根律\ 定理}
$$\left(\bigcup\limits_{\alpha}^{}E_\alpha\right)^C =\  \bigcap\limits_{\alpha}^{}(E_\alpha^C)$$
$$\left(\bigcap\limits_{\alpha}^{}E_\alpha\right)^C =\  \bigcup\limits_{\alpha}^{}(E_\alpha^C)$$
